WIP: alternative proof of strong normalization, following Lemma 3.2.1

theories/SimplyTypedLambdaCalculus/StrongNormalisation.v
@@ -1,4 +1,5 @@
 From FormArith.SimplyTypedLambdaCalculus Require Import Definitions.
+Import List.ListNotations.
 
 
 Inductive SN: term -> Prop :=
@@ -73,6 +74,353 @@ Proof.
   now inversion 1.
 Qed.
 
+Fixpoint atomic' (t: term):=
+  match t with 
+  | Var _ => True (* unsure if this case should be included or not? *)
+  | App l _ => atomic' l
+| _ => False
+  end.
+
+Definition atomic (t: term) := atomic' t /\ SN t.
+
+Lemma SN_subst (t: term) (σ: var -> term):
+  SN t -> forall (u: term), t = u.[σ] -> SN u.
+Proof.
+  induction 1 as [? _ IHt]; intros; subst.
+
+  apply Strong.
+  intros t ?.
+
+  apply IHt with t.[σ].
+  - now apply beta_subst.
+  - reflexivity.
+Qed.
+
+(*Lemma 3.2.1 (3) refers to terms of this specific shape*)
+Fixpoint nested_app t l :=
+  match l with 
+  | nil => t
+  | cons t' l' => App (nested_app t l') t'
+  end.
+
+Lemma atomic_step t s : atomic' t -> t ->β s -> atomic' s.
+Proof.
+  induction t in s |- *; cbn.
+  - inversion 2.
+  - intros Hat Hstep. inversion Hstep; subst.
+    + contradiction.
+    + cbn. apply IHt1; assumption.
+    + cbn. assumption.
+  - tauto.
+Qed.
+
+Lemma atomic_app_r t u : atomic t -> SN u -> atomic (App t u).
+Proof.
+  intros [Hat Hsnt] Hsnu.
+  split.
+  - tauto.
+  - induction Hsnt in Hat, u, Hsnu |-*.
+    induction Hsnu in H0 |- *.
+    constructor. intros t' Hstep.
+    inversion Hstep; subst.
+    + contradiction.
+    + apply H0.
+      * assumption.
+      * eapply atomic_step; eassumption.
+      * constructor. assumption.
+    + apply H2. 1: assumption. assumption.
+Qed.
+
+Lemma SN_ind_pair (P : term -> term -> Prop):
+  (forall t u, (forall t' u', ((t = t' /\ u ->β u') \/ (t ->β t' /\ u = u')) -> P t' u') -> P t u)
+    -> forall t u, SN t -> SN u -> P t u.
+Proof.
+  intros IH ? ? Hsnt.
+  revert u.
+
+  induction Hsnt as [? _ IHt].
+  intros ? Hsnt.
+
+  induction Hsnt as [? ? IHv].
+  apply IH.
+
+  intros ? ? [[? ?] | [? ?]]; subst.
+  - now apply IHv.
+  - apply IHt; [ assumption |].
+    now apply Strong.
+Qed.
+
+(*
+  Enumerate all the possible next steps of a term.
+  This is helpful (and probably only helpful) for the max_steps lemma.
+*)
+Fixpoint enumerate_steps (t : term) : list term :=
+  match t with 
+  | Var _ => []
+  | Lam s => List.map Lam (enumerate_steps s)
+  | App s t => List.map (fun s => App s t) (enumerate_steps s)
+                ++ List.map (fun t => App s t) (enumerate_steps t)
+                ++ match s with
+                   | Lam s' => [s'.[t/]]
+                   | __ => []
+                   end
+  end.
+
+(*
+  enumerate_steps is sound and complete:
+ *)
+Lemma enumerate_steps_spec t: forall t', List.In t' (enumerate_steps t) <-> t ->β t'.
+Proof.
+  induction t as [x | s IHs t IHt | s IHs].
+  - intros u; cbn. split.
+    + firstorder.
+    + inversion 1.
+  - intros u; cbn. split.
+    + intros Hin. apply List.in_app_or in Hin as [Hin | Hin]. 2: apply List.in_app_or in Hin as [Hin | Hin].
+      * rewrite List.in_map_iff in Hin. destruct Hin as  [s' [<- Hs']].
+        apply IHs in Hs'.
+        now constructor.
+      * rewrite List.in_map_iff in Hin. destruct Hin as [t' [<- Ht']].
+        apply IHt in Ht'.
+        now constructor.
+      * destruct s; try firstorder.
+        now constructor.
+    + intros Hstep. inversion Hstep; subst.
+      * apply List.in_or_app. right. apply List.in_or_app. right.
+        firstorder.
+      * apply List.in_or_app. left.
+        apply (List.in_map (fun s' => App s' t)).
+        now apply IHs.
+      * apply List.in_or_app. right. apply List.in_or_app. left.
+        apply (List.in_map (fun t' => App s t')).
+        now apply IHt.
+  - intros u; cbn. split.
+    + intros Hin. apply List.in_map_iff in Hin.
+      destruct Hin as [s' [<- Hs']].
+      apply IHs in Hs'.
+      now constructor.
+    + inversion 1; subst.
+      apply List.in_map. now apply IHs.
+Qed.
+
+(*
+  This version is slightly nicer to use in the following proof:
+*)
+Lemma enumerate_Forall_beta t : List.Forall (fun t' => t ->β t') (enumerate_steps t).
+Proof.
+  apply List.Forall_forall.
+  apply enumerate_steps_spec.
+Qed.
+
+(*
+  reduction_sequences are lists where any element beta-reduces to the next element.
+  This helps us reason about the number of reduction steps any term can take.
+ *)
+Fixpoint reduction_sequence (l : list term) : Prop :=
+  match l with 
+  | nil => True
+  | cons t nil => True
+  | cons s (cons t l' as ll) => s ->β t /\ reduction_sequence ll
+  end.
+
+Require Import Lia.
+
+(*
+  Any strongly normalizing term has a maximum number of steps it can reduce.
+  We state this by stating a maximal length for any reduction sequence.
+
+  Intuitively, this is by induction on SN, which gives us the induction hypothesis for each possible next step.
+   The correctness proof follows since for any reduction sequence starting in t and with first step t', the remaining sequence must be a reduction sequence for t', so the induction hypothesis applies.
+  In practice, it is much more difficult, since we need to determine the maximum of the (existentially quantified) numbers of steps for each next term.
+*)
+Lemma max_steps (t: term) : SN t -> exists n, forall l, reduction_sequence (t :: l) -> length l <= n.
+Proof.
+  (*The proof is by induction on SN, which is also why we can't (easily) state this as a function.*)
+  intros Hsn. induction Hsn as [t Hsn IH].
+  (*First, we apply the induction hypothesis to all terms in `enumerate_steps` (i.e. all the terms t can reduce to).*)
+  assert (List.Forall (fun t' => t ->β t' /\ exists n, forall l, reduction_sequence (t' :: l) -> length l <= n) (enumerate_steps t)) as H.
+  + pose proof (enumerate_Forall_beta t) as H.
+    induction H.
+    * constructor.
+    * constructor. 2: assumption.
+      firstorder.
+  + (*Unfortunately, the maximal lengths for all t' are currently hidden underneath existential quantifiers, and not easily accessible.
+      We begin by moving them into an existentially quantified list.*)
+    assert (exists l', length l' = length (enumerate_steps t) /\ List.Forall (fun (p : term * nat) => let (t', n) := p in forall l, reduction_sequence (t' :: l) -> length l <= n) (List.combine (enumerate_steps t) l')) as [l' [Hlen Hl']].
+    * induction H as [|t' l Ht' HForall IHForall].
+      -- exists nil. firstorder.
+      -- destruct Ht' as [_ [n Hn]].
+         destruct IHForall as [l' Hl'].
+         exists (cons n l').
+         split.
+         ++ cbn. firstorder.
+         ++ constructor; firstorder.
+    * (* We now have l', the list of the maximal number of steps for each term in `enumerate_steps t`.*)
+      (* Clearly, we need at least one more step:*)
+      exists (S(List.list_max l')).
+      clear - l' Hlen Hl'.
+      (* For the correctness proof, we inspect the reduction sequence:*)
+      intros l Hred.
+      destruct l as [|t' l]. 1: cbn; lia. (*empty reduction sequences are trivial.*)
+      (* The first step in the reduction sequence must be a valid reduction step, so we must also have the next term in enumerate_steps.
+         Intuitively, we should thus be able to apply Hl'; but this requires some more difficulty:
+      *)
+      destruct Hred as [Hbeta Hred].
+      rewrite <- enumerate_steps_spec in Hbeta.
+      (* We first need to obtain the index of t', so that we can recover its associated number of steps.*)
+      apply List.In_nth with (d := Var 0) in Hbeta. destruct Hbeta  as (ind & Hind & Hbeta).
+      pose (List.nth ind l' 0) as n'.
+      (* n' is the max number of steps of t', but we need to recover this fact.
+         It is stored in Hl', so we need to instantiate the `Forall` with the corresponding index:
+      *)
+      pose (List.nth ind (List.combine (enumerate_steps t) l') (Var 0, 0)) as p.
+      assert (p = (t', n')) as Heq by (subst; now apply List.combine_nth).
+      assert (List.In p (List.combine (enumerate_steps t) l')) as Hp.
+      { apply List.nth_In.
+        pose proof (List.combine_length (enumerate_steps t) l').
+        lia.
+      }
+      rewrite List.Forall_forall in Hl'. apply Hl' in Hp.
+      rewrite Heq in Hp.
+      (* After all this, we have recovered what is essentially the induction hypothesis for t'.
+        Since (t :: t' :: l) is a valid reduction sequence for t, (t' :: l) must be a valid reduction sequence for t'; thus, the IH applies.
+       *)
+      specialize (Hp l).
+      assert (n' <= List.list_max l'). (*This is more or less the definition of list_max, but apparently, it is not in the library directly?*)
+      { assert (List.list_max l' <= List.list_max l') as H by constructor.
+        rewrite List.list_max_le in H.
+        rewrite List.Forall_forall in H.
+        apply H.
+        apply List.nth_In. congruence.
+      }
+      apply Hp in Hred.
+      cbn. lia.
+Qed.
+
+(* The standard strong induction on natural numbers *)
+Lemma nat_strong_ind:
+  forall P: nat -> Prop, (forall n, (forall m, m < n -> P m) -> P n) -> forall n, P n.
+Proof.
+  intros P Hind n.
+  enough (forall m, m <= n -> P m) as H.
+  - apply H. constructor.
+  - induction n.
+    + intros m. destruct m.
+      * intros _. apply Hind.
+        lia.
+      * lia.
+    + intros m Hm.
+      inversion Hm.
+      * subst. apply Hind.
+        intros m' Hm'.
+        apply IHn. lia.
+      * subst. now apply IHn.
+Qed.
+
+(* Lemma 3.2.1 statement (3) for the base case, where the entire term is of some atomic type.
+   Formalizing this proof is difficult:
+   While intuitively, any reduction step is either within any subterm (not changing the specified shape) or reduction of the leftmost application,
+   the main difficulty in Coq stems from the fact that we do not know the size of the term (i.e. the number of applications).
+
+   The current attempt uses the maximal numbers of steps (as determined by max_steps),
+   but is stuck at destructing the actual reduction step. Presumably, induction is needed, but I have not yet found a version that yields suitable induction hypotheses.
+*)
+Lemma base_case t u l : SN (nested_app t.[u/] l) -> SN u -> forall t', nested_app (App (Lam t) u) l ->β t' -> SN t'.
+Proof.
+  intros Hsn Hsnu.
+  (*determine the maximum number of steps for t*)
+  assert (exists nt, forall l, reduction_sequence (t :: l) -> length l <= nt) as [nt Hnt].
+  { admit. } (*chore: we don't have a lemma to do this yet, so induction on l?*)
+  (*determine the maximum number of steps for u*)
+  assert (exists nu, forall l, reduction_sequence (u :: l) -> length l <= nu) as [nu Hnu].
+  { apply max_steps. assumption. }
+  (*determine the maximum number of steps for all terms in l*)
+  assert (exists l', length l' = length l /\ List.Forall (fun (p : term * nat) => let (t, n) := p in forall l, reduction_sequence (t :: l) -> length l <= n) (List.combine l l')) as [l' Hl'].
+  { induction l.
+    - exists nil; firstorder.
+    - cbn in Hsn.
+      assert (SN a) as Ha.
+      { eapply SN_sub_term. 1: exact Hsn. constructor. }
+      assert (SN (nested_app t.[u/] l)) as Hsn'.
+      { eapply SN_sub_term. 1: exact Hsn. constructor. }
+      specialize (IHl Hsn').
+      destruct IHl as [l' Hl'].
+      apply max_steps in Ha.
+      destruct Ha as [n Hn].
+      exists (cons n l').
+      cbn. firstorder.
+  }
+  (*We wish to do induction on the sum of all these step numbers: This will allow us to use the induction hypothesis for any step in any of these terms.*)
+  remember (nt + nu + List.list_sum l') as n.
+  (*We do induction on n with everything else quantified.*)
+  induction n as [n IH] using nat_strong_ind in t, u, l, Hsn, Hsnu, nt, Hnt, nu, Hnu, l', Hl', Heqn |- *.
+  intros t' Hstep.
+
+  (*below, my current best attempt at doing this proof, using induction on the derivation of the step. However, the induction hypothesis is not of a suitable shape.*)
+  (*some subgoals are marked as chore and admitted: they should be provable but just require a bit of work.*)
+  remember (nested_app (App (Lam t) u) l) as trm.
+  induction Hstep in t, u, l, Hsn, Hsnu, nt, Hnt, nu, Hnu, l', Hl', Heqn, Heqtrm |- *.
+  - subst.
+    destruct l.
+    + cbn in Heqtrm. inversion Heqtrm; subst. exact Hsn.
+    + cbn in Heqtrm. inversion Heqtrm; subst.
+      destruct l; cbn in *; congruence.
+  - subst.
+    (* this _should_ be an application of IHHstep somehow, but the hypothesis is not of the right shape.
+       this may be doable by strengthening the statement to wrap it in another nested_app, then proving things about nested_app and append?
+    *)
+    admit.
+  - destruct l.
+    + cbn in Heqtrm. inversion Heqtrm; subst.
+      admit. (*chore*)
+    + cbn in Heqtrm. inversion Heqtrm; subst.
+      destruct l'. 1: cbn in *; firstorder; congruence.
+      change (SN (nested_app (App (Lam t) u) (t' :: l))).
+      eapply IH with (l := cons t1 l).
+      8: now constructor.
+      2-5: eassumption.
+      3: reflexivity.
+      (*chore : since t1 ->β t', there is an n' < n with the desired property; instantiate ?l' with n'::l'. the second subgoal will be annoying.*)
+      all: admit.
+  - destruct l; cbn in Heqtrm; congruence.
+Admitted.
+
+(*Lemma 3.2.1 of the lecture notes.*)
+Lemma reducible_is_SN_variant_1 (A : type):
+  (forall (t: term), reducible A t -> SN t) /\
+  (forall (t: term), atomic t -> reducible A t) /\
+  (forall (t u: term) l, reducible A (nested_app (t.[u .: ids]) l) -> SN u -> reducible A (nested_app (App (Lam t) u) l)).
+Proof.
+  induction A as [ | A1 IHA1 A2 IHA2 ].
+  - split. 2: split.
+    (*the first two statements are easy in the base case.*)
+    + intros t Ht. constructor. intros t'.
+      apply SN_inverted. assumption.
+    + intros t [_ Hsnt]. now destruct Hsnt.
+    + intros t u l H Hsnu. cbn in *. 
+      constructor.
+      (*the third statement is very difficult: see above.*)
+      now apply base_case.
+  - split. 2: split.
+    + cbn. intros t Hred.
+      apply SN_sub_term with (t := App t (Var 0)).
+      2: constructor.
+      apply IHA2, Hred.
+      apply IHA1. split. 
+      * cbn. tauto.
+      * constructor. intros ? H. inversion H.
+    + cbn. intros t Hat u Hred.
+      apply IHA2. split.
+      * apply Hat.
+      * apply IHA1 in Hred.
+        apply atomic_app_r; assumption.
+    + intros t u l Hred Hsnu u' Hred'.
+      change (reducible A2 (nested_app (App (Lam t) u) (cons u' l))).
+      apply IHA2.
+      * cbn. now apply Hred.
+      * assumption.
+Qed.
+
 Lemma reducible_is_SN (A : type):
   (forall (t: term), reducible A t -> SN t) /\
     (forall (t u: term), reducible A t -> t ~> u -> reducible A u) /\
@@ -118,19 +466,6 @@ Proof.
       * now apply Hredt.
       * apply IHu; [ assumption |].
         now apply IHA2 with u.
-Qed.
-
-Lemma SN_subst (t: term) (σ: var -> term):
-  SN t -> forall (u: term), t = u.[σ] -> SN u.
-Proof.
-  induction 1 as [? _ IHt]; intros; subst.
-
-  apply Strong.
-  intros t ?.
-
-  apply IHt with t.[σ].
-  - now apply beta_subst.
-  - reflexivity.
 Qed.
 
 Lemma SN_ind_pair (P : term -> term -> Prop):
